\documentclass[12pt]{article}
\usepackage{graphicx} % Required for inserting images
\usepackage[letter, margin=0.5in]{geometry}
\usepackage{amsmath}


\setcounter{secnumdepth}{0} % Removes section numbering


\date{\vspace{-4ex}}


\title{Physical Mechanics HW1}
\author{Damien Koon}

\begin{document}

\maketitle

\centering{(1). For the two vectors:}

\centering{$\vec{A} = \hat{i} + 2\hat{j} - \hat{k}$} 

\centering{$\vec{B} = -2\hat{i} + 3\hat{j} + \hat{k}$}

\hfill \break

(a) $\vec{A} - \vec{B}$ and $|\vec{A} - \vec{B}|$

\hfill \break

$
\vec{A} - \vec{B} = (1-(-2))\hat{i} + (2 - 3)\hat{j} + (-1 - 1)\hat{k} = \boldsymbol{3\hat{i} - \hat{j} -2\hat{k}}
$ 

$
|\vec{A} - \vec{B}| =  \sqrt{(3)^2 + (-1)^2 + (-2)^2} = \sqrt{9 + 1 + 4} = \boldsymbol{\sqrt{14}}
$

\hfill \break

(b) The component of $\vec{B}$ along $\vec{A}$ 

$
\hat{A} = \frac{A}{|A|} = \frac{\hat{i} + 2\hat{j} - \hat{k}}{\sqrt{6}} \rightarrow Comp_{\vec{B}} \vec{A} = \vec{B} \cdot \hat{A} = \frac{-2 + 6 - 1}{\sqrt{6}} = \boldsymbol{\frac{\sqrt{6}}{2}}
$

\hfill \break

(c) The angle between $\vec{A}$ and $\vec{B}$

$
\vec{A} \cdot \vec{B} = |A||B|cos(\theta) \rightarrow \theta = cos^{-1}(\frac{\vec{A} \cdot \vec{B}}{|A||B|}) = cos^{-1}(\frac{-2 + 6 -1}{\sqrt{6} \sqrt{14}}) = cos^{-1}(\frac{\sqrt21}{14}) = \boldsymbol{70.89^{\circ}}
$

\hfill \break

(d) $\vec{A} \times \vec{B}$

$$
\begin{bmatrix}
    \hat{i} & \hat{j} & \hat{k} \\
	1 & 2 & -1\\
	-2 & 3 & 1 \\
\end{bmatrix}
= \hat{i}
\begin{bmatrix}
	2 & -1\\
	3 & 1 \\
\end{bmatrix}
- \hat{j}
\begin{bmatrix}
	1 & -1\\
	-2 & 1 \\
\end{bmatrix}
+ \hat{k}
\begin{bmatrix}
	1 & 2\\
	-2 & 3 \\
\end{bmatrix}
= (2 + 3)\hat{i} - (1 - 2) \hat{j} + (3 + 4) \hat{k} 
$$
$$
= \boldsymbol{5\hat{i} + \hat{j} + 7 \hat{k}}
$$

\hfill \break


(e) $(\vec{A} - \vec{B}) \times (\vec{A} + \vec{B})$

\hfill \break

$
(\vec{A} - \vec{B}) = 3\hat{i} - \hat{j} -2\hat{k}
$

$
\vec{A} + \vec{B} = (1+(-2))\hat{i} + (2 + 3)\hat{j} + (-1 + 1)\hat{k} = -\hat{i} + 5\hat{j}
$

$$
\begin{bmatrix}
    \hat{i} & \hat{j} & \hat{k} \\
	3 & -1 & -2\\
	-1 & 5 & 0 \\
\end{bmatrix}
= \hat{i}
\begin{bmatrix}
	-1 & -2\\
	5 & 0 \\
\end{bmatrix}
- \hat{j}
\begin{bmatrix}
	3 & -2\\
	-1 & 0 \\
\end{bmatrix}
+ \hat{k}
\begin{bmatrix}
	3 & -1\\
	-1 & 5 \\
\end{bmatrix}
= (0 + 7)\hat{i} - (0 - 2) \hat{j} + (15 - 1) \hat{k} 
$$
$$
= \boldsymbol{7\hat{i} + 2\hat{j} + 14 \hat{k}}
$$


(2). A particle moves in a plane elliptical orbit described by the position vector:

\large\centering{$\vec{r} = 2bsin(\omega t) \hat{i} + bcos(\omega t) \hat{j} $}

\hfill \break

(a) Find $\vec{v}, \vec{a}, $ and the particle's speed.

$$
\vec{v} = \frac{d \vec{r}}{dt} = \frac{d}{dt}[2bsin(\omega t) \hat{i} + bcos(\omega t) \hat{j}] = \boldsymbol{2b \omega cos(\omega t) \hat{i} - b\omega sin(\omega t) \hat{j}}
$$

$$
\vec{a} = \frac{d \vec{v}}{dt} = \frac{d}{dt}[2b \omega cos(\omega t) \hat{i} - b\omega sin(\omega t) \hat{j}] = \boldsymbol{ -2b \omega^2 sin(\omega t) \hat{i} - b\omega^2 cos(\omega t) \hat{j} }
$$

$$
|\vec{v}| = v = \sqrt{(2b \omega cos(\omega t))^2 + (-b\omega sin(\omega t))^2} = \sqrt{4b^2 \omega^2 cos^2(\omega t) + b^2 \omega^2 sin^2(\omega t)}
$$

$
v = \boldsymbol{b \omega \sqrt{4cos^2(\omega t) + sin^2(\omega t)}}
$

\hfill \break



(b) What is the angle between $\vec{v}$ and $\vec{a}$ at $t=\frac{\pi}{2\omega}$

$$
\vec{v}(t) = 2b \omega cos(\omega t) \hat{i} - b\omega sin(\omega t) \hat{j} \rightarrow \vec{v}(\frac{\pi}{2\omega}) = 2b \omega cos(\frac{\pi}{2}) \hat{i} - b\omega sin(\frac{\pi}{2}) \hat{j}
$$

$$
\vec{v}(\frac{\pi}{2\omega}) = \sqrt{2}b\omega \hat{i} - b\omega \frac{\sqrt{2}}{2} \hat{j}= b \omega 2\sqrt{2} ((2\hat{i} - \hat{j})
$$

$$
|\vec{v}(\frac{\pi}{2\omega})| = \sqrt{8b^{2}\omega^{2}(4 + 1)} = 2b\omega \sqrt{10}
$$

$$
\vec{a}(t) = -2b \omega^2 sin(\omega t) \hat{i} - b\omega^2 cos(\omega t) \hat{j} \rightarrow \vec{a}(\frac{\pi}{2\omega}) = -2b \omega^2 sin(\frac{\pi}{2}) \hat{i} - b\omega^2 cos(\frac{\pi}{2}) \hat{j}
$$
$
\vec{a}(\frac{\pi}{2\omega}) = -2b\omega^{2}\sqrt{2}(2\hat{i}+\hat{j})
$

$$
|\vec{a}(\frac{\pi}{2\omega})| = \sqrt{8b^{2}\omega^{4}(4+1)} = 2b\omega^{2} \sqrt{10}
$$

$$
\vec{a} \cdot \vec{v} = (b\omega 4\sqrt{2} * -b\omega^{2} 4\sqrt{2}) + (-b\omega 2\sqrt{2} * -b\omega^{2} 2\sqrt{2}) = (-32b^{2}\omega^{3} + 8b^{2} \omega^{3}) = -26b^2\omega^3
$$

$$
\vec{a} \cdot \vec{v} = |\vec{a}||\vec{v}|cos(\theta) \rightarrow \theta = cos^{-1}(\frac{\vec{a} \cdot \vec{v}}{|\vec{a}||\vec{v}|})
$$

$$
\theta = cos^{-1}(\frac{-26b^2\omega^3}{2b\omega^{2} \sqrt{10} * 2b\omega \sqrt{10}}) = cos^{-1}(\frac{-26}{40}) = \boldsymbol{130.542^{\circ}}
$$

\hfill \break

(3). $\vec{X}$ is an unknown vector satisfying the following relations involving the known vectors $\vec{A}$ and $\vec{B}$ and the scalar $\phi$. Express $\vec{X}$ in terms of $\vec{A}, \vec{B}, \phi, |A|$ 

$$
\vec{A} \times \vec{X} = \vec{B}
$$

$
\vec{A} \cdot \vec{X} = \phi
$


$$
\vec{A} \times \vec{X} = \vec{B} \rightarrow \vec{A} \times (\vec{A} \times \vec{X}) = \vec{A} \times \vec{B}
$$
Using
$$
\vec{A} \times (\vec{B} \times \vec{C}) = \vec{B}(\vec{A} \cdot \vec{C}) - \vec{C}(\vec{A} \cdot \vec{B})
$$

$$
\vec{A} \times (\vec{A} \times \vec{X}) = \vec{A} \times \vec{B} = \vec{A}(\vec{A} \cdot \vec{X}) - \vec{X}(\vec{A} \cdot \vec{A}) = \vec{A} \times \vec{B}
$$

$$
\vec{A} \phi - \vec{X} A^2 = \vec{A} \times \vec{B}
$$

$$
\boldsymbol{\vec{X} = \frac{\vec{A} \phi - \vec{A} \times \vec{B}}{A^2}}
$$


\newpage


(4) Recover the cosine law of plane trigonometry (a.k.a. the law of cosines) by interpreting the product $(\vec{A} - \vec{B}) \cdot (\vec{A} - \vec{B})$ and the expansion of the product.

\hfill \break

\ell et 

$\vec{C} = \vec{A} - \vec{B}$

$$
\vec{A} - \vec{B} \cdot \vec{A} - \vec{B} = \vec{C} \cdot \vec{C} = C^2
$$

$$
C^2 = (\vec{A} - \vec{B}) \cdot \vec{C} = (\vec{A} \cdot \vec{C}) - (\vec{B} \cdot \vec{C})
$$

$$
C^2 = (\vec{A} \cdot (\vec{A} - \vec{B})) - (\vec{B} \cdot (\vec{A} - \vec{B})
$$

$$
C^2 = \vec{A} \cdot \vec{A} - \vec{A} \cdot \vec{B} - \vec{B} \cdot \vec{A} + \vec{B} \cdot \vec{B}
$$

$$
C^2 = A^2 + B^2 - (\vec{A} \cdot \vec{B} + \vec{B} \cdot \vec{A})
$$

$$
C^2 = A^2 + B^2 - (ABcos(\theta) + BAcos(\theta))
$$

$$
\boldsymbol{C^2 = A^2 + B^2 - 2ABcos(\theta)}
$$


\end{document}
